finished the homomorphism proof.
- required an addition to meaning of a homomorphism.

theories/RecordTableaux.v
@@ -1,4 +1,5 @@
 Require Import Coq.Lists.List.
+Require Import ExtLib.Tactics.
 Require Import SemanticQuery.Tables.
 
 Set Implicit Arguments.
@@ -25,12 +26,42 @@ Section with_tables.
     | t :: ts , u :: us => f t u :: join f ts us
     end.
 
+  Fixpoint cross {T U V : Type} (f : T -> U -> V) (ts : list T) (us : list U) : list V :=
+    match ts with
+    | nil => nil
+    | t :: ts => List.map (f t) us ++ cross f ts us
+    end.
+
+
+  Lemma In_cross : forall {T U V} (f : T -> U -> V) us ts,
+      forall x,
+        In x (cross f ts us) <->
+        exists t u,
+          In t ts /\ In u us /\ x = f t u.
+  Proof.
+    induction ts; simpl; intros.
+    { split.
+      { inversion 1. }
+      { intros.
+        forward_reason. assumption. } }
+    { rewrite List.in_app_iff.
+      rewrite IHts; clear IHts.
+      rewrite in_map_iff.
+      split; intros; forward_reason.
+      { destruct H; forward_reason.
+        { subst. do 2 eexists; eauto. }
+        { do 2 eexists; eauto. } }
+      { destruct H; subst.
+        { left; eauto. }
+        { right. eauto. } } }
+  Qed.
+
   Fixpoint bindD {ts : list row_type} (names : hlist (fun x => member x tbls) ts)
     : hlist table tbls -> list (hlist row ts) :=
     match names in hlist _ ts return hlist table tbls -> list (hlist row ts) with
     | Hnil => fun _ => Hnil :: nil
     | Hcons _ _ n names => fun tbls =>
-                             join (fun a b => Hcons a b) (hlist_get n tbls) (bindD names tbls)
+                             cross (fun a b => Hcons a b) (hlist_get n tbls) (bindD names tbls)
     end.
 
   Fixpoint exprD {T} {ls} (e : expr T ls) {struct e} : hlist row ls -> type T :=
@@ -94,38 +125,192 @@ Section with_tables.
       @existT2 _ _ _ T (f x1) (f x2)
     end.
 
-  (*
-    A homomorphism h : t1 -> t2 maps the for-bound variables of t1 to the for-bound variables of t2 such that
-    1) x in X in t1 implies h(x) in X in t2
-    2) t1 |- p = q in t1 implies t2 |- h(p) = h(q)
-    3) return E in t1 and return E' in t2 implies t2 |- h(E) = E'
-   *)
-  Definition tableaux_homomorphism (t1 t2 : tableaux) : Type :=
-  { h : forall x, member x t1.(types) -> member x t2.(types) (** 1 **)
-  & forall x, filterD (map (subst_test (subst_expr h)) t1.(filter)) x = filterD t2.(filter) x (** 2? **)
-  }.
-
-  Definition query_homomorphism ts (q1 q2 : query ts) : Type :=
-  { th : tableaux_homomorphism q1.(tabl) q2.(tabl)
-  & forall r, filterD (map (subst_test (subst_expr (projT1 th))) q1.(tabl).(filter)) r = true ->
-              retD (hlist_map (fun T (x : expr T (types q1.(tabl))) => subst_expr (projT1 th) _ x) q1.(ret)) r =
-              retD q2.(ret) r
-  }.
-
   Definition list_set_subset {T} (a b : list T) : Prop :=
     forall x, In x a -> In x b.
 
   Definition list_set_equiv {T} (a b : list T) : Prop :=
     list_set_subset a b /\ list_set_subset b a.
 
+
+  (*
+    A homomorphism h : t1 -> t2 maps the for-bound variables of t1 to the for-bound variables of t2 such that
+    1) x in X in t1 implies h(x) in X in t2
+    2) t1 |- p = q in t1 implies t2 |- h(p) = h(q)
+    3) return E in t1 and return E' in t2 implies t2 |- h(E) = E'
+   *)
+  Definition types_homomorphism (ts1 ts2 : list row_type) : Type :=
+    forall x : row_type, member x ts1 -> member x ts2.
+  Definition binds_homomorphism {ts1 ts2 : list row_type}
+             (h : types_homomorphism ts1 ts2)
+             (b1 : hlist (fun x => member x tbls) ts1)
+             (b2 : hlist (fun x => member x tbls) ts2) : Type :=
+    forall t (x : member t _), hlist_get x b1 = hlist_get (h _ x) b2.
+  Definition filter_homomorphism {ts1 ts2 : list row_type}
+             (h : types_homomorphism ts1 ts2)
+             (f1 : list { T : dec_type & expr T ts1 & expr T ts1 })
+             (f2 : list { T : dec_type & expr T ts2 & expr T ts2 }) : Type :=
+    forall x, filterD (map (subst_test (subst_expr h)) f1) x = filterD f2 x.
+
+  Record tableaux_homomorphism (t1 t2 : tableaux) : Type :=
+  { vars_mor : types_homomorphism t1.(types) t2.(types)
+  ; bindsOk  : binds_homomorphism vars_mor t1.(binds) t2.(binds) (** 1 **)
+  ; filterOk : filter_homomorphism vars_mor t1.(filter) t2.(filter) (** 2 **)
+  }.
+
+  Record query_homomorphism ts (q1 q2 : query ts) : Type :=
+  { th : tableaux_homomorphism q1.(tabl) q2.(tabl)
+  ; retOk : forall r, filterD (map (subst_test (subst_expr th.(vars_mor))) q1.(tabl).(filter)) r = true ->
+              retD (hlist_map (fun T (x : expr T (types q1.(tabl))) => subst_expr th.(vars_mor) _ x) q1.(ret)) r =
+              retD q2.(ret) r
+  }.
+
+  Definition related {ts1 ts2 : list row_type} (h : forall x : row_type, member x ts1 -> member x ts2)
+             (b1 : hlist row ts1)
+             (b2 : hlist row ts2) : Prop :=
+    forall t (m : member t ts1),
+      hlist_get m b1 = hlist_get (h _ m) b2.
+
+  Lemma In_bindD_hlist_get
+    : forall (l : row_type) (ts2 : list row_type) (tbl_data : hlist table tbls)
+             (b2 : hlist (fun x : row_type => member x tbls) ts2)
+             (x : hlist row ts2)
+             (m : member l ts2),
+      In x (bindD b2 tbl_data) ->
+      In (hlist_get m x) (hlist_get (hlist_get m b2) tbl_data).
+  Proof.
+    induction b2.
+    { simpl. intros. inversion m. }
+    { simpl. intros.
+      eapply In_cross in H. forward_reason.
+      subst.
+      destruct (member_case m); forward_reason.
+      { subst. simpl. auto. }
+      { subst. simpl. eauto. } }
+  Qed.
+
+  Lemma bindD_subset
+    : forall ts1 (b1 : hlist (fun x => member x tbls) ts1)
+             ts2 (b2 : hlist (fun x => member x tbls) ts2),
+      forall tbl_data x,
+        In x (bindD b2 tbl_data) ->
+        forall (h : types_homomorphism ts1 ts2),
+          binds_homomorphism h b1 b2 ->
+          exists y,
+            related h y x /\
+            In y (bindD b1 tbl_data).
+  Proof.
+    induction b1.
+    { intros. exists Hnil.
+      simpl. split; eauto.
+      red. clear. intros. inversion m. }
+    { simpl. intros.
+      setoid_rewrite In_cross.
+      specialize (IHb1 _ _ _ _ H (fun t m => h t (MN _ m))).
+      match goal with
+      | H : ?X -> _ |- _ =>
+        cut X;
+          [ let H' := fresh in
+            intro H' ; specialize (H H') | ]
+      end.
+      { forward_reason.
+        exists (Hcons (hlist_get (h _ (MZ _ _)) x) x0).
+        split.
+        { red. intros.
+          destruct (member_case m).
+          { destruct H3. subst. simpl. reflexivity. }
+          { forward_reason. subst. simpl. eauto. } }
+        { do 2 eexists; split; eauto.
+          red in X. red in H0.
+          specialize (X l (MZ l ls)).
+          simpl in X. subst.
+          eauto using In_bindD_hlist_get. } }
+      { revert X. clear. unfold binds_homomorphism.
+        intros. eapply (X t (MN _ x)). } }
+  Qed.
+
+  Lemma related_exprD_subst_expr
+  : forall (types0 types1 : list row_type)
+           (vars_mor0 : types_homomorphism types1 types0)
+           (x0 : hlist row types0) (x : hlist row types1),
+      related vars_mor0 x x0 ->
+      forall (x1 : dec_type) (e : expr x1 types1),
+        exprD (subst_expr vars_mor0 x1 e) x0 = exprD e x.
+  Proof.
+    induction e.
+    { simpl. red in H.
+      f_equal. symmetry. eapply H. }
+  Qed.
+
+  Lemma related_filterD_subst_test
+    : forall (ts : list dec_type) (q1 : query ts) (tabl0 : tableaux)
+             (vars_mor0 : types_homomorphism (types tabl0) (types (tabl q1)))
+             (x0 : hlist row (types (tabl q1))) (x : hlist row (types tabl0)),
+      related vars_mor0 x x0 ->
+      forall
+        l : list {T : dec_type & expr T (types tabl0) & expr T (types tabl0)},
+        filterD l x = filterD (map (subst_test (subst_expr vars_mor0)) l) x0.
+  Proof.
+    induction l; simpl; auto.
+    { destruct a; simpl.
+      rewrite <- IHl.
+      do 2 erewrite related_exprD_subst_expr by eauto.
+      reflexivity. }
+  Qed.
+
+  Lemma retD_related
+    : forall (types1 types0 : list row_type)
+             (x0 : hlist row types1) (x : hlist row types0)
+             (vars_mor0 : types_homomorphism types0 types1),
+      related vars_mor0 x x0 ->
+      forall (ts : list dec_type)
+             (ret0 : hlist (fun t : dec_type => expr t types0) ts),
+        retD ret0 x =
+        retD
+          (hlist_map
+             (fun (T : dec_type) (x1 : expr T types0) => subst_expr vars_mor0 T x1)
+             ret0) x0.
+  Proof.
+    induction ret0; simpl; auto.
+    f_equal.
+    { erewrite related_exprD_subst_expr; eauto. }
+    { eassumption. }
+  Qed.
+
   Lemma homomorphism_subset ts
     : forall q1 q2,
-      @query_homomorphism ts q1 q2 ->
+      @query_homomorphism ts q2 q1 ->
       forall tbls,
         list_set_subset (queryD q1 tbls) (queryD q2 tbls).
   Proof.
     unfold queryD, tableauxD.
-    admit.
+    destruct 1. red.
+    intros.
+    eapply List.in_map_iff in H.
+    eapply List.in_map_iff.
+    forward_reason.
+    eapply List.filter_In in H0.
+    setoid_rewrite List.filter_In.
+    forward_reason.
+    eapply bindD_subset in H0.
+    2: eapply bindsOk.
+    revert H0; instantiate (4 := th0); intro H0.
+    subst. forward_reason.
+    destruct th0; simpl in *.
+    exists x. split; [ | split ].
+    { rewrite <- retOk0.
+      { destruct q2. simpl in *. clear - H.
+        destruct q1. simpl in *. clear - H.
+        destruct tabl0; destruct tabl1. simpl in *.
+        eauto using retD_related. }
+      { rewrite <- H1.
+        red in filterOk0.
+        rewrite <- filterOk0. reflexivity. } }
+    { assumption. }
+    { red in filterOk0. clear retOk0 bindsOk0.
+      rewrite <- filterOk0 in H1.
+      rewrite <- H1.
+      destruct q2. simpl in *.
+      eapply related_filterD_subst_test; eauto. }
   Qed.
 
   Theorem bihomomorphism_equal ts
